Common/Reduction.lean
@@ -1,4 +1,5 @@
 
 import Common.Reduction.Definition
 import Common.Reduction.Basic
+import Common.Reduction.Plus
 import Common.Reduction.Confluence
