Fomega/Basic/Weaken.lean
@@ -69,11 +69,16 @@ namespace Fomega.Proof
     case _ => apply ih3 r h1 h2
     case _ => apply ih4 r h1 h2
   case fst ih =>
-    simp; constructor; case _ => apply ih r h1 h2
+    simp; constructor; apply ih r h1 h2
   case snd ih =>
-    simp; constructor; case _ => apply ih r h1 h2
-  case id ih =>
-    simp; apply Judgment.id; case _ => apply ih r h1 h2
+    simp; constructor; apply ih r h1 h2
+  case unit ih =>
+    simp; constructor; apply ih r h1 h2
+  case unit_ty ih =>
+    simp; constructor; apply ih r h1 h2
+  case unit_rec ih1 ih2 ih3 =>
+    simp; constructor; apply ih1 r h1 h2
+    apply ih2 r h1 h2; apply ih3 r h1 h2
   case conv Γ' t A' B K _j1 _j2 j3 ih1 ih2 =>
     constructor
     case _ => apply ih1 r h1 h2
