WCCC/FomegaModel/Consistency.lean
@@ -1,0 +1,19 @@
+
+import WCCC.Proof
+import WCCC.Proof.Derivations
+import Fomega.Basic.Derivations
+import WCCC.FomegaModel.Interpretation
+import WCCC.FomegaModel.Normalization
+
+namespace FomegaModel
+
+  theorem equational_consistency
+    : ¬ ([] ⊢c t : .eq cBool ctt cff)
+  := by sorry
+
+  theorem logical_consistency
+    : ¬ ([] ⊢c t : cFalse)
+  := by sorry
+
+
+end FomegaModel
